setting up tactics

Lgtm/Hyper/ProofMode.lean
@@ -9,6 +9,7 @@ import Lgtm.Unary.WP1
 import Lgtm.Hyper.YSimp
 import Lgtm.Hyper.YChange
 import Lgtm.Hyper.WP
+import Lgtm.Hyper.WPUtil
 import Lgtm.Hyper.Subst
 import Lgtm.Hyper.Arrays
 import Lgtm.Hyper.HProp
@@ -66,8 +67,13 @@ macro_rules
 macro "WP [" n:num "|" i:ident " in " s:term " => " t:lang "]" ppSpace Q:term : term =>
   `(hwp ⟪$n,$s⟫ (fun $i:ident => [lang|$t]) $Q)
 
+macro "WP [" n:num "|" i:ident " in " s:term " => " t:lang "]"  "{ " v:ident ", " Q:term " }" : term =>
+  `(hwp ⟪$n,$s⟫ (fun $i:ident => [lang|$t]) fun $v => $Q)
+
+
 @[app_unexpander hwp] def unexpandHWP : Lean.PrettyPrinter.Unexpander
-  | `($(_) ⟪$n:num,$s⟫ (fun $i:ident => [lang|$t])) => `(WP [$n| $i in $s => $t] ⋯)
+  | `($(_) ⟪$n:num,$s⟫ (fun $i:ident => [lang|$t])) => do
+    `(WP [$n| $i in $s => $t] ⋯)
   | _ => throw ( )
 
 -- #check LGTM.SHT.mk
@@ -76,7 +82,7 @@ macro_rules
 
 @[app_unexpander LGTM.SHT.mk] def unexpandSHT : Lean.PrettyPrinter.Unexpander :=
   fun x => match x with
-  | `($(_) ⟪$n:num,$s⟫ fun $i:ident => [lang|$t]) => `([sht| [$n | $i in $s => $t] ])
+  | `($(_) ⟪$n:num,$s⟫ fun $i:ident => [lang|$t]) => do `([sht| [$n | $i in $s => $t] ])
   | `({ s:= ⟪$n:num,$s⟫, ht := (fun $i:ident ↦ [lang|$t]) }) => `([sht| [$n | $i in $s => $t] ])
   | _ => throw ( )
 
@@ -91,9 +97,13 @@ macro_rules
   | _ => throw ( )
 
 @[app_unexpander hwp] def unexpandLGTMWP : Lean.PrettyPrinter.Unexpander
-  | `($(_) ⟪$n:num,$s⟫ $f $_) =>
+  | `($(_) ⟪$n:num,$s⟫ $f fun $_ => NWP $_* { $_, $_ }) =>
     match f with
     | `(fun $i:ident => [lang|$t]) => `(WP [$n| $i in $s => $t] ⋯)
+    | _ => throw ( )
+  | `($(_) ⟪$n:num,$s⟫ $f fun $v:ident => $Q) =>
+    match f with
+    | `(fun $i:ident => [lang|$t]) => `(WP [$n| $i in $s => $t] { $v:ident, $Q:term })
     | _ => throw ( )
   | _ => throw ( )
 
@@ -113,21 +123,21 @@ macro_rules
 
 /- --- Lemmas for focus/unfocus --- -/
 
--- class FindLabel (l : LabType) (sht : LGTM.SHTs (Labeled α)) (i : outParam ℕ)
---   (_ : outParam (i < sht.length)) where
---   findLabel : ∃ s, sht[i].s = ⟪l, s⟫
+class FindLabel (l : LabType) (sht : LGTM.SHTs (Labeled α)) (i : outParam ℕ)
+  (_ : outParam (i < sht.length)) where
+  findLabel : ∃ s, sht[i].s = ⟪l, s⟫
 
--- instance (priority := high) FindLabelHead : FindLabel l (⟨⟪l,s⟫, ht⟩ :: shts) 0 (by simp) where
---   findLabel := by move=> ⟨|⟩//
+instance (priority := high) FindLabelHead : FindLabel l (⟨⟪l,s⟫, ht⟩ :: shts) 0 (by simp) where
+  findLabel := by move=> ⟨|⟩//
 
--- instance FindLabelTail (shts : LGTM.SHTs (Labeled α)) (pi : i < shts.length)
---   [inst: FindLabel l shts i pi] :
---   FindLabel l (⟨⟪l',s⟫, ht⟩ :: shts) (i+1) (by simp; omega) where
---   findLabel := by scase: inst=> [s] /== ->; exists s=> //
+instance FindLabelTail (shts : LGTM.SHTs (Labeled α)) (pi : i < shts.length)
+  [inst: FindLabel l shts i pi] :
+  FindLabel l (⟨⟪l',s⟫, ht⟩ :: shts) (i+1) (by simp; omega) where
+  findLabel := by scase: inst=> [s] /== ->; exists s=> //
 
-lemma xfocus_lemma (l : LabType) (shts : LGTM.SHTs (Labeled α)) {pi : l-1 < shts.length} :
+lemma yfocus_lemma (l : LabType) (shts : LGTM.SHTs (Labeled α)) {pi} [FindLabel l shts i pi] :
   (List.Pairwise (Disjoint ·.s ·.s) shts) ->
-  LGTM.wp shts Q = hwp shts[l-1].s shts[l-1].ht fun hv => LGTM.wp (shts.eraseIdx (l-1)) (Q $ hv ∪_shts[l-1].s ·) := by
+  LGTM.wp shts Q = hwp shts[i].s shts[i].ht fun hv => LGTM.wp (shts.eraseIdx i) (Q $ hv ∪_shts[i].s ·) := by
   apply LGTM.wp_focus
 
 lemma List.insertNth_getElem (l : List α) {_ : j <= l.length}
@@ -144,29 +154,29 @@ lemma List.eraseIdx_getElem (l : List α) {_ : j + 1 < l.length}
   (l.eraseIdx i)[j] = if h : j < i then l[j]'(by omega) else l[j+1]'(by omega) := by
   sorry
 
-lemma xunfocus_lemma (l : LabType) (shts : LGTM.SHTs (Labeled α)) {pi : l-1 < shts.length}
+lemma yunfocus_lemma (idx : ℕ) (l : LabType) (shts : LGTM.SHTs (Labeled α)) {pi : idx < shts.length}
   (Q' : hval (Labeled α) -> hval (Labeled α) -> hhProp (Labeled α)):
   (shts.Pairwise (Disjoint ·.s ·.s)) ->
   (shts.Forall (Disjoint ⟪l,s⟫ ·.s)) ->
   (∀ hv hv', Q' hv hv' = Q (hv ∪_⟪l, s⟫ hv')) ->
   hwp ⟪l,s⟫ ht (fun hv => LGTM.wp shts fun hv' => Q' hv hv') =
-  LGTM.wp (shts.insertNth (l-1) ⟨⟪l, s⟫, ht⟩) Q := by
-  move=> dj dj' Qeq; srw (xfocus_lemma l)
+  LGTM.wp (shts.insertNth idx ⟨⟪l, s⟫, ht⟩) Q := by
+  move=> dj dj' Qeq; srw (LGTM.wp_focus idx)
   { srw List.getElem_insertNth_self //= List.eraseIdx_insertNth /=
     congr! 4=> //' }
   srw List.pairwise_iff_getElem at dj
   srw List.forall_iff_forall_mem at dj'
   srw List.pairwise_iff_getElem=> > ?
   srw ?(List.insertNth_getElem shts) //'
-  { scase: [i < l - 1]=> ?
+  { scase: [i < idx]=> ?
     { srw dif_neg //' [2]dif_neg; rotate_left; omega
-      scase: [i = l-1]=> [?|?]
+      scase: [i = idx]=> [?|?]
       { srw dif_neg //' dif_neg; rotate_left; omega
         apply dj; omega }
       srw dif_pos //' /= dif_neg; rotate_left; omega
       apply dj'; apply List.getElem_mem }
-    srw dif_pos //';  scase: [j < l-1]=> [?|?]
-    { srw dif_neg //'; scase: [j = l-1]=> ?
+    srw dif_pos //';  scase: [j < idx]=> [?|?]
+    { srw dif_neg //'; scase: [j = idx]=> ?
       { srw dif_neg //'; apply dj; omega }
       srw dif_pos //' /= disjoint_comm; apply dj'; apply List.getElem_mem
       srw List.length_insertNth at _hi <;> omega }
@@ -187,18 +197,19 @@ abbrev fun_lab_insert (l : LabType) (f g : Labeled α -> β) :=
   fun x => if x.lab = l then f x else g x
 -- (_ \ _) ∪ (_ ∩ _)
 set_option maxHeartbeats 1600000 in
-lemma xfocus_set_lemma_aux (l : LabType) (s' s : Set α) (shts : LGTM.SHTs (Labeled α)) {pi : l-1 < shts.length} :
-  shts[l-1].s = ⟪l, s⟫ ->
+lemma yfocus_set_lemma_aux (idx : ℕ) (l : LabType) (s' s : Set α) (shts : LGTM.SHTs (Labeled α))
+  {pi : idx < shts.length} :
+  shts[idx].s = ⟪l, s⟫ ->
   (shts.Pairwise (Disjoint ·.s ·.s)) ->
-  (Disjoint (LGTM.SHTs.set (List.eraseIdx shts (l - 1))) ⟪l, Set.univ⟫) ->
-    (hwp ⟪l, s \ s'⟫ shts[l-1].ht fun hv =>
-    LGTM.wp ((shts.eraseIdx (l-1)).insertNth (l-1) ⟨⟪l, s ∩ s'⟫,shts[l-1].ht⟩) fun hv' =>
+  (Disjoint (LGTM.SHTs.set (List.eraseIdx shts idx)) ⟪l, Set.univ⟫) ->
+    (hwp ⟪l, s \ s'⟫ shts[idx].ht fun hv =>
+    LGTM.wp ((shts.eraseIdx (idx)).insertNth idx ⟨⟪l, s ∩ s'⟫,shts[idx].ht⟩) fun hv' =>
       Q $ fun_lab_insert l (hv' ∪_⟪l,s'⟫ hv) hv') ==> LGTM.wp shts Q := by
     move=> seq /[dup]?/List.pairwise_iff_getElem dj' /[dup] dj₁ /Set.disjoint_left dj
-    srw (xfocus_lemma l) //' seq -(Set.diff_union_inter ⟪l,s⟫ ⟪l,s'⟫) /==
+    srw (LGTM.wp_focus idx) //' seq -(Set.diff_union_inter ⟪l,s⟫ ⟪l,s'⟫) /==
     srw hwp_union; apply hwp_conseq=> //'; rotate_left
     { simp [disjE, Set.disjoint_sdiff_inter] }
-    move=> hv₁ /=; srw (xfocus_lemma l)
+    move=> hv₁ /=; srw (LGTM.wp_focus idx)
     { srw  List.getElem_insertNth_self //=; rotate_left
       { srw List.length_eraseIdx //' }
       srw List.eraseIdx_insertNth /=
@@ -219,8 +230,8 @@ lemma xfocus_set_lemma_aux (l : LabType) (s' s : Set α) (shts : LGTM.SHTs (Labe
     rotate_left
     { srw List.length_eraseIdx=> //' }
     srw ?(List.insertNth_getElem _) //'
-    { scase: [i < l - 1]=> ?
-      { srw dif_neg //'; scase: [i = l -1]=> ?
+    { scase: [i < idx]=> ?
+      { srw dif_neg //'; scase: [i = idx]=> ?
         { srw dif_neg //' (List.eraseIdx_getElem _) <;> try omega
           sdo 3 srw dif_neg <;> try omega
           srw (List.eraseIdx_getElem _) <;> try omega
@@ -235,8 +246,8 @@ lemma xfocus_set_lemma_aux (l : LabType) (s' s : Set α) (shts : LGTM.SHTs (Labe
         srw getElem!_pos //'  (List.eraseIdx_getElem _) //'
         srw dif_neg //' }
       srw dif_pos //' (List.eraseIdx_getElem _) //' dif_pos //'
-      scase: [j < l - 1]=> ?
-      { srw dif_neg //'; scase: [j = l - 1]=> ?
+      scase: [j < idx]=> ?
+      { srw dif_neg //'; scase: [j = idx]=> ?
         { srw dif_neg //' (List.eraseIdx_getElem _) //' dif_neg //'
           apply dj'=> //' }
         srw dif_pos //'=> /=; apply Set.disjoint_of_subset _ _ dj₁=> x //'
@@ -246,31 +257,52 @@ lemma xfocus_set_lemma_aux (l : LabType) (s' s : Set α) (shts : LGTM.SHTs (Labe
       srw dif_pos //'(List.eraseIdx_getElem _) //' }
     all_goals srw List.length_eraseIdx=> //'
 
-lemma xfocus_set_lemma (l : LabType) (s' s : Set α) (shts : LGTM.SHTs (Labeled α)) {pi : l-1 < shts.length} :
-  shts[l-1].s = ⟪l, s⟫ ->
+lemma yfocus_set_lemma (l : LabType) (s' s : Set α) (shts : LGTM.SHTs (Labeled α)) {pi : idx < shts.length}
+  [FindLabel l shts idx pi] :
+  shts[idx].s = ⟪l, s⟫ ->
   (shts.Pairwise (Disjoint ·.s ·.s)) ->
-  (Disjoint (LGTM.SHTs.set (List.eraseIdx shts (l - 1))) ⟪l, Set.univ⟫) ->
-    H ==> (hwp ⟪l, s \ s'⟫ shts[l-1].ht fun hv =>
-    LGTM.wp ((shts.eraseIdx (l-1)).insertNth (l-1) ⟨⟪l, s ∩ s'⟫,shts[l-1].ht⟩) fun hv' =>
+  (Disjoint (LGTM.SHTs.set (List.eraseIdx shts idx)) ⟪l, Set.univ⟫) ->
+    H ==> (hwp ⟪l, s \ s'⟫ shts[idx].ht fun hv =>
+    LGTM.wp ((shts.eraseIdx idx).insertNth idx ⟨⟪l, s ∩ s'⟫,shts[idx].ht⟩) fun hv' =>
       Q $ fun_lab_insert l (hv' ∪_⟪l,s'⟫ hv) hv') -> H ==> LGTM.wp shts Q := by
-  move=> *; apply hhimpl_trans_r; apply xfocus_set_lemma_aux=> //
+  move=> *; apply hhimpl_trans_r; apply yfocus_set_lemma_aux=> //
+
+lemma yclean_up_lemma (l : LabType) (s : Set α)
+  (shts : LGTM.SHTs (Labeled α)) (Q : hval (Labeled α) -> hhProp (Labeled α)) :
+  (shts.Forall (Disjoint ⟪l,Set.univ⟫ ·.s)) ->
+  (forall hr, Q' hr = Q (v ∪_⟪l, s⟫ hr)) ->
+  H ==> LGTM.wp shts (fun hr => Q (fun_lab_insert l v hr)) ->
+  H ==> LGTM.wp shts Q' := by
+  move=> dj Qeq h; ychange h; apply hwp_conseq'=> hv /=
+  ysimp [fun_lab_insert l v hv]; srw Qeq;
+  apply congr_hhimpl; congr!; funext ⟨m, x⟩=> /==
+  scase_if=> //== ?; scase_if; scase_if=> //
+  srw shts_set_eq_sum /== => ??
+  srw getElem!_pos //;
+  srw List.forall_iff_forall_mem Set.disjoint_left /== at dj
+  move=> /dj f; exfalso; apply f=> //; apply List.getElem_mem
+
+lemma ywp1 :
+  LGTM.wp [⟨s, ht⟩] = hwp s ht := by
+  move=> !Q; srw LGTM.wp /==; apply hwp_ht_eq=> ?? //
 
 
 open Lean Elab Tactic Meta Qq
 
 attribute [-simp] fun_insert
-macro "xfocus" n:num : tactic => do
-  `(tactic| (erw [xfocus_lemma $n:term]=> /=; ⟨skip, simp, try simp [disjE]⟩))
+macro "yfocus" n:num : tactic => do
+  `(tactic| (erw [yfocus_lemma $n:term]=> /=; ⟨skip, try simp [disjE]⟩))
 
-macro "xfocus" n:num ", " s:term : tactic => do
-  `(tactic| (apply xfocus_set_lemma $n:term $s=> /=;
-             ⟨try simp [disjE], try simp [disjE], skip, try auto⟩
+macro "yfocus" n:num ", " s:term : tactic => do
+  `(tactic| (apply yfocus_set_lemma $n:term $s=> /=;
+             ⟨try simp [disjE], try simp [disjE], skip⟩
    ))
 
 set_option linter.unreachableTactic false in
 set_option linter.unusedTactic false in
-elab "xunfocus" : tactic => do
-  {| srw xunfocus_lemma /== |}
+elab "yunfocus" n:num ? : tactic => do
+  let n := n.getD (<- `(num|1))
+  {| srw (yunfocus_lemma ($n-1)) /== |}
   let gs <- getUnsolvedGoals
   let [gRest, gDj, gQeq, _] := gs | failure
   /- try to resolve disjointness -/
@@ -284,28 +316,381 @@ elab "xunfocus" : tactic => do
   gQen.refl
   setGoals [gRest]
 
+macro "ycleanup" n:num : tactic => do
+  `(tactic|
+    (apply (yclean_up_lemma $n);
+     ⟨simp [disjE],
+      (move=> ?
+       generalize (_ ∪_⟪$n, _⟫ _) = x; rfl),
+      (dsimp; try srw ywp1), skip, skip, skip⟩))
 
-instance (α : Type*) : Coe (Labeled α) α where
-  coe l := l.val
+macro "yin " n:num ":" colGe ts:tacticSeq : tactic =>
+  `(tactic| (
+    yfocus $n;
+    ($ts) <;> try (first | yunfocus $n |ycleanup $n)))
+
+--   ))
+
+
+/- ################################################################# -/
+/-* * Practical Proofs -/
+
+/-* This last section shows the techniques involved in setting up the lemmas
+    and tactics required to carry out verification in practice, through
+    concise proof scripts. -/
+
+/- ================================================================= -/
+/-* ** Lemmas for Tactics to Manipulate [wpgen] Formulae -/
+
+lemma ystruct_lemma (F : @hformula α) H Q :
+  H ==> F Q →
+  H ==> hmkstruct F Q := by
+  move=> h
+  ychange h
+  unfold hmkstruct
+  ysimp
+
+lemma yval_lemma v H (Q : hval α -> hhProp α) :
+  H ==> Q v →
+  H ==> hwpgen_val v Q := by
+  move=> h
+  ychange h
+
+lemma ylet_lemma H (F1 : @hformula α) F2of Q :
+  H ==> F1 (fun v => F2of v Q) →
+  H ==> hwpgen_let F1 F2of Q :=
+by
+  move=> h
+  ychange h
+
+lemma yseq_lemma H (F1 F2 : @hformula α) Q :
+  H ==> F1 (fun _ => F2 Q) →
+  H ==> hwpgen_seq F1 F2 Q :=
+by
+  move=> h
+  ychange h
+
+lemma xif_lemma b H F1 F2 Q :
+  (b = true -> H ==> F1 Q) →
+  (b = false -> H ==> F2 Q) →
+  H ==> hwpgen_if (fun (_ : htrm α) => b) F1 F2 Q :=
+by
+  scase: b
+  move=> /== h
+  sby all_goals ychange h ; unfold hwpgen_if ; ysimp
+
+lemma yapp_lemma : forall t Q1 H1 H Q,
+  htriple s t H1 Q1 ->
+  H ==> H1 ∗ (Q1 -∗ protect Q) ->
+  H ==> hwpgen_app s t Q :=
+by
+  move=> T M
+  unfold hwpgen_app=> ?????
+  ysimp
+  apply htriple_ramified_frame=> //
+
+
+lemma ywp_lemma_fun (v1 v2 : hval α) (x : α -> var) (t : htrm α) H Q :
+  (∀ i, v1 i = val_fun (x i) (t i)) →
+  H ==> hwp s (fun i => subst (x i) (v2 i) (t i)) Q →
+  htriple s (fun x => trm_app (v1 x) (v2 x)) H Q :=
+by sorry
+
+lemma ywp_lemma_fix : forall (v1 v2 : hval α) (f x : α -> var) (t : htrm α) H Q,
+  (∀ i, v1 i = val_fix (f i) (x i) (t i)) ->
+  f != x ->
+  H ==> hwp s (fun i => subst (x i) (v2 i) $ subst (f i) (v1 i) $ (t i)) Q ->
+  htriple s (fun i => trm_app (v1 i) (v2 i)) H Q :=
+by sorry
+
+lemma ytriple_lemma t H (Q:hval α → hhProp α) :
+  H ==> hmkstruct (hwpgen_app s t) Q →
+  htriple s t H Q :=
+by
+  move=> M
+  srw -hwp_equiv
+  ychange M
+  unfold hmkstruct hwpgen_app
+  ypull=> >
+  srw -hwp_equiv => N
+  ychange N
+  apply hwp_ramified
+
+
+/- ================================================================= -/
+/-* ** Tactics to Manipulate [wpgen] Formulae -/
+
+/-* The tactic are presented in chapter [WPgen]. -/
+
+/- [xstruct] removes the leading [mkstruct]. -/
+
+section tactics
+
+open Lean Elab Tactic
+
+macro "ystruct" : tactic => do
+  `(tactic| apply ystruct_lemma)
+
+
+set_option linter.unreachableTactic false in
+set_option linter.unusedTactic false in
+elab "ystruct_if_needed" : tactic => do
+  match <- getGoalStxAll with
+  | `($_ ==> hmkstruct $_ $_) => {| apply ystruct_lemma |}
+  | _ => pure ( )
+macro "ylet" : tactic => do
+  `(tactic| (ystruct_if_needed; apply ylet_lemma; dsimp))
+
+macro "yseq" : tactic => do
+  `(tactic| (ystruct_if_needed; apply yseq_lemma))
+
+set_option linter.unreachableTactic false in
+set_option linter.unusedTactic false in
+elab "yseq_xlet_if_needed" : tactic => do
+  match <- getGoalStxAll with
+  | `($_ ==> hwpgen_let $_ $_ $_) => {| ylet |}
+  | `($_ ==> hwpgen_seq $_ $_ $_) => {| yseq |}
+  | _ => pure ( )
+
+macro "yif" : tactic => do
+  `(tactic|
+  (yseq_xlet_if_needed; ystruct_if_needed; apply yif_lemma))
+
+set_option linter.unreachableTactic false in
+set_option linter.unusedTactic false in
+elab "yapp_try_clear_unit_result" : tactic => do
+  let .some (_, _) := (← Lean.Elab.Tactic.getMainTarget).arrow? | pure ( )
+  -- let_expr val := val | pure ()
+  {| move=> _ |}
+
+macro "ytriple" :tactic =>
+  `(tactic| (intros; apply ytriple_lemma))
+
+set_option linter.unreachableTactic false in
+set_option linter.unusedTactic false in
+elab "ywp_equiv" :tactic => do
+  let_expr hhimpl _ _ wp := (<- getMainTarget) | pure ( )
+  let_expr hwp _ _ _ _ := wp | pure ( )
+  {| rw [hwp_equiv] |}
+
+
+set_option linter.unreachableTactic false in
+set_option linter.unusedTactic false in
+elab "ytriple_if_needed" : tactic => do
+  let_expr htriple _ _ _ _ _ := (<- getMainTarget) | pure ( )
+  {| ytriple |}
+
+lemma yapp_simpl_lemma (F : hformula) :
+  H ==> F Q ->
+  H ==> F Q ∗ (Q -∗ protect Q) := by sorry
+
+elab "ysimp_step_no_cancel" : tactic => do
+  let ysimp <- YSimpRIni
+  /- TODO: optimise.
+    Sometimes we tell that some transitions are not availible at the moment.
+    So it might be possible to come up with something better than trying all
+    transitions one by one -/
+  withMainContext do
+    ysimp_step_l  ysimp false <|>
+    ysimp_step_r  ysimp <|>
+    ysimp_step_lr ysimp
+
+macro "ysimp_no_cancel_wand" : tactic =>
+  `(tactic| (
+    ysimp_start
+    repeat' ysimp_step_no_cancel
+    try rev_pure
+    try hsimp
+  ))
+
+section yapp
+
+macro "ywp" : tactic =>
+  `(tactic|
+    (intros
+     first | apply ywp_lemma_fix; rfl
+           | apply ywp_lemma_fun; rfl))
+
+macro "yapp_simp" : tactic => do
+  `(tactic|
+      first | apply yapp_simpl_lemma; try hsimp
+            | ysimp_no_cancel_wand; try unfold protect; yapp_try_clear_unit_result)
+
+macro "yapp_pre" : tactic => do
+  `(tactic|
+    (yseq_xlet_if_needed
+     ywp_equiv
+     ytriple_if_needed
+     ystruct_if_needed))
+
+set_option linter.unreachableTactic false in
+set_option linter.unusedTactic false in
+elab "yapp_try_subst" : tactic => do
+  {| (unhygienic (skip=>>)
+      move=>->) |}
+
+macro "yapp_debug" :tactic => do
+  `(tactic|
+    (yapp_pre
+     eapply yapp_lemma))
+
+set_option linter.unreachableTactic false in
+set_option linter.unusedTactic false in
+
+elab "yapp_pick" e:term ? : tactic => do
+  let thm <- (match e with
+    | .none => pickHTripleLemma
+    | .some thm => return thm.raw.getId : TacticM Name)
+  {| eapply $(mkIdent thm) |}
+
+set_option linter.unreachableTactic false in
+set_option linter.unusedTactic false in
+-- elab "yapp_nosubst"  : tactic => do
+--   {| (yapp_pre
+--       eapply yapp_lemma; yapp_pick_debug
+--       rotate_left; yapp_simp=>//) |}
+
+macro "yapp_nosubst" e:term ? : tactic =>
+  `(tactic|
+    (yapp_pre
+     eapply yapp_lemma; yapp_pick $(e)?
+     rotate_right; yapp_simp; hide_mvars=>//))
+
+macro "yapp" : tactic =>
+  `(tactic|
+    (yapp_nosubst;
+     try yapp_try_subst
+     first
+       | done
+       | all_goals try srw hwp_equiv
+         all_goals try subst_vars))
+
+elab "yapp" colGt e:term ? : tactic => do
+  {|
+    (yapp_nosubst $(e)?;
+     try yapp_try_subst
+     first
+       | done
+       | all_goals try srw hwp_equiv
+         all_goals try subst_vars) |}
+
+end yapp
+
+
+end tactics
+
+@[simp]
+abbrev var_funs (xs:List var) (n:Nat) : Prop :=
+     xs.Nodup
+  /\ xs.length = n
+  /\ xs != []
+
+@[simp]
+def trms_vals (vs : List var) : List trm :=
+  vs.map trm_var
+
+instance : Coe (List var) (List trm) where
+  coe := trms_vals
+
+-- lemma trms_vals_nil :
+--   trms_vals .nil = .nil := by rfl
+@[simp]
+def trms_to_vals (ts:List trm) : Option (List val) := do
+  match ts with
+  | [] => return []
+  | (trm_val v) :: ts' => v :: (<- trms_to_vals ts')
+  | _ => failure
+
+/- ======================= WP Generator ======================= -/
+/- Below we define a function [wpgen t] recursively over [t] such that
+   [wpgen t Q] entails [wp t Q].
+
+   We actually define [wpgen E t], where [E] is a list of bindings, to
+   compute a formula that entails [wp (isubst E t)], where [isubst E t]
+   is the iterated substitution of bindings from [E] inside [t].
+-/
+
+open AList
+
+-- abbrev ctx := AList (fun _ : var ↦ val)
+
+/- Definition of Multi-Substitution -/
+
+
+lemma trm_apps1 :
+  trm_app t1 t2 = trm_apps t1 [t2] := by rfl
+
+lemma trm_apps2 :
+  trm_apps (trm_app t1 t2) ts = trm_apps t1 (t2::ts) := by rfl
+
+
+lemma ywp_lemma_funs (xs : α -> List var) (vs : α -> List val) (t t1 : htrm α)
+  (ts : α -> List trm):
+  (∀ i, t i = trm_apps (v0 i) (ts i)) ->
+  (v0 = fun i => val_funs (xs i) (t1 i)) ->
+  (∀ i, trms_to_vals (ts i) = vs i) ->
+  (∀ i, var_funs (xs i) (vs i).length) ->
+  H ==> hwp s (fun i => Unary.isubst ((xs i).mkAlist (vs i)) $ t1 i) Q ->
+  htriple s t H Q := by sorry
+
+lemma xwp_lemma_fixs (xs : α -> List var) (vs : α -> List val) (t t1 : htrm α)
+  (ts : α -> List trm) (f : α -> var) :
+  (∀ i, t i = trm_apps (v0 i) (ts i)) ->
+  (v0 = fun i => val_fixs (f i) (xs i) (t1 i)) ->
+  (∀ i, trms_to_vals (ts i) = (vs i)) ->
+  (∀ i, var_funs (xs i) (vs i).length) ->
+  (∀ i, f i ∉ (xs i)) ->
+  H ==> hwp s (fun i => Unary.isubst ((f i :: xs i).mkAlist (v0 i :: vs i)) $ t1 i) Q ->
+  htriple s t H Q := by sorry
+
+-- lemma wp_of_wpgen :
+--   H ==> wpgen t Q →
+--   H ==> wp t Q := by sorry
+
+
+macro "ywp" : tactic =>
+  `(tactic|
+    (intros
+     try simp_rw [trm_apps1]
+     repeat simp_rw [trm_apps2]
+     try (first | (apply ywp_lemma_fixs; rfl; rfl; sdone; sdone; sdone)=> //'
+                | (apply ywp_lemma_funs; rfl; rfl; rfl; sdone)=> //')
+     apply hwp_of_hwpgen
+     all_goals try simp
+       [hwpgen,
+        subst,
+        isubst, trm_apps, AList.lookup, List.dlookup]
+     all_goals try simp [_root_.subst, trm_apps]))
+
+macro "yval" : tactic => do
+  `(tactic| (ystruct_if_needed; yseq_xlet_if_needed; (try ywp); apply yval_lemma))
+
 
 section
 
 variable {H : hhProp (Labeled Int)}
 
+instance : Coe (Labeled ℤ) ℤ where
+  coe l := l.val
 
-#check [sht| [1 | i in {1,3} => let x := ⟨i.val⟩ in x + 1] ]
+-- #check [sht| [1 | i in {(1 : ℤ),3} => let x := ⟨i⟩ in x + 1] ]
 example :
-  H ∗ H ==>
-    NWP [1 | i in {1,3} => let x := ⟨i⟩ in x + 1]
+  emp ==>
+    NWP [1 | i in {(1 : ℤ),3} => let x := ⟨i⟩ in x + 1]
         [2 | i in {1,3} => let x := ⟨i⟩ in x + 1]
-    { v, ⌜v ⟨1,1⟩ = 2 ∧ v ⟨2,1⟩ = 2 ∧ v ⟨1,1⟩ = 2⌝ } := by
-  xfocus 1; xunfocus
-  xfocus 2, {3}=> /==
-  sorry
-#check
-  { (H ∗ H) }
-    [1 | i in {1,3} => let x := ⟨i⟩ in x + 1]
-    [2 | i in {1,3} => let x := ⟨i⟩ in x + 1]
-  { v, ⌜v ⟨1,1⟩ = 2 ∧ v ⟨1,1⟩ = 2 ∧ v ⟨1,1⟩ = 2⌝ }
+    { v, ⌜v ⟨1,1⟩ = 2 ∧ v ⟨2,1⟩ = 2 ∧ v ⟨1,3⟩ = 4⌝ } := by
+  yin 1: ywp; yval
+  yfocus 2, {3}=> /==
+  ywp; yval
+  yapp htriple_add
+  yin 2: ywp; yval; yapp htriple_add
+  yapp htriple_add
+  srw fun_insert /==; ysimp
+
+-- #check
+--   { (H ∗ H) }
+--     [1 | i in {1,3} => let x := ⟨i.val⟩ in x + 1]
+--     [2 | i in {1,3} => let x := ⟨i.val⟩ in x + 1]
+--   { v, ⌜v ⟨1,1⟩ = 2 ∧ v ⟨1,1⟩ = 2 ∧ v ⟨1,1⟩ = 2⌝ }
 
 end
